<setup>
<selectFromSequence name="a" from="2" to="5"/>
<selectFromSequence name="c" from="-3" to="3"/>  
<function name="f">
    $a*x - x^2
  </function>
  <derivative name="fP">$f</derivative>  
</setup>

  <p>
    Consider the function <m>f(x) = $f</m>.  We are going to use the limit definition of the derivative to determine <m>f'($c)</m>.

    <ol marker="a.">
      <li>
        <p>
          Recall that the limit definition of <m>f'($c)</m> is
          <me> f'($c) = \lim_{h \to 0} \frac{f($c+h)-f($c)}{h} </me>
          and thus we need to determine expressions for <m>f($c+h)</m> and <m>f($c+h) - f($c)</m>.
        </p>

        <p>Using the given formula <m>f(x) = $f</m>, 
      which of the following is the simplest possible expression for <m>f($c+h)</m>?</p>
            <answer>
              <choiceInput>
                <choice><m>f($c+h) = $a($c+h)-($c+h)^2 </m></choice>
                <choice><m>f($c+h)=  - h^2 + <math simplify> $c($a-$c) + $a*h </math></m>  </choice>
                <choice><m>f($c+h)=   h^2 + <math simplify> $c($a-$c) + ($a-2$c)*h </math></m>  </choice>
                <choice credit="1"><m>f($c+h)=   -h^2 + <math simplify> $c($a-$c) + ($a-2$c)*h </math></m>  </choice> 
              </choiceInput>
            </answer>  
      </li>
      <li>
      <p>Which of the following is the simplest possible expression for <m>f($c+h) - f($c)</m>?</p>
            <answer>
              <choiceInput>
                <choice><m>f($c+h) - f($c) = $a($c+h)-($c+h)^2 + <math simplify>-1*$$f($c)</math> </m></choice>
                <choice><m>f($c+h) - f($c) =  - h^2 + <math simplify>$a*h </math></m>  </choice>
                <choice credit="1"><m>f($c+h)  - f($c) =   -h^2 + <math simplify> ($a-2$c)*h </math></m>  </choice> 
                <choice><m>f($c+h) - f($c) =   h^2 + <math simplify>($a-2$c)*h </math></m>  </choice>  
              </choiceInput>
            </answer>   
      </li>
      <li> Next, apply the limit definition of the derivative by substituting the simplest possible expression for <m>f($c+h)-f($c)</m> in the space provided:
        <p><m>f'($c)= \displaystyle \lim_{h \to 0} \frac{f($c+h)-f($c)}{h} = \lim_{h \to 0} </m> <mathInput name="dq_x1" prefill="/h"></mathInput>
      <answer><award><when>$dq_x1 = 
        ($$f($c+h) - $$f($c))/h
      </when></award></answer></p>
      </li>
      <li>
        <p>Further, factoring the numerator and simplifying, we see that</p>
        <p>  <m>f'($c)= \displaystyle \lim_{h \to 0} </m> <mathInput name="simp_x1"></mathInput>
      <answer><award><when>$simp_x1 = 
        ($$f($c+h) - $$f($c))/h
      </when></award></answer></p>
      </li>
      <li>
        <p>Finally, evaluating the limit by letting <m>h \to 0</m>, we determine the value of <m>f'($c)</m>:</p>
        <p><m>f'($c) = </m> <answer>$$fP($c)</answer></p>
      </li>

    </ol>
  </p>